Finish sequence and trying to verify non-trivial test props.

src/asn1/ASN1.Spec.TLV.Specialized.fst
@@ -6,10 +6,12 @@ open ASN1.Spec.Length
 open ASN1.Spec.BOOLEAN
 open ASN1.Spec.NULL
 open ASN1.Spec.OCTET_STRING
+open ASN1.Spec.SEQUENCE
 open LowParse.Bytes
 
-module I = FStar.Integers
+open FStar.Integers
 
+/// Interface
 let parse_asn1_TLV_kind_of_type
   (_a: asn1_primitive_type)
 : parser_kind
@@ -34,128 +36,86 @@ let serialize_asn1_TLV_of_type
   | NULL         -> serialize_asn1_null_TLV
   | OCTET_STRING -> serialize_asn1_octet_string_TLV
 
-/// Ad-hoc sequence parser/serializer
-///
+// let parse_asn1_TLV_of_type_unfold
+//   (_a: asn1_primitive_type)
+// : GTot (bytes -> _)
+// = match _a with
+//   | BOOLEAN      -> (parse_asn1_boolean_TLV_unfold)
+//   | NULL         -> (parse_asn1_null_TLV_unfold)
+//   | OCTET_STRING -> (parse_asn1_octet_string_TLV_unfold)
 
-let parse_asn1_sequence_TL_kind
-: parser_kind
-= parse_asn1_tag_kind
-  `and_then_kind`
-  parse_asn1_length_kind_of_type SEQUENCE
+// let serialize_asn1_TLV_of_type_unfold
+//   (_a: asn1_primitive_type)
+// : GTot (datatype_of_asn1_type _a -> _)
+// = match _a with
+//   | BOOLEAN      -> (serialize_asn1_boolean_TLV_unfold)
+//   | NULL         -> (serialize_asn1_null_TLV_unfold)
+//   | OCTET_STRING -> (serialize_asn1_octet_string_TLV_unfold)
 
-let parse_asn1_sequence_TL
-: parser parse_asn1_sequence_TL_kind (the_asn1_type SEQUENCE & asn1_int32_of_type SEQUENCE)
-= parse_the_asn1_tag SEQUENCE
-  `nondep_then`
-  parse_asn1_length_of_type SEQUENCE
-
-let serialize_asn1_sequence_TL
-: serializer parse_asn1_sequence_TL
-= serialize_the_asn1_tag SEQUENCE
-  `serialize_nondep_then`
-  serialize_asn1_length
 
 #push-options "--query_stats --z3rlimit 32"
 let safe_add
   (a b: option asn1_int32)
-: Tot (option asn1_int32)
+: Tot (c: option asn1_int32 {
+          Some?a /\ Some?b /\ Some? c ==>
+            v (Some?.v c) == v (Some?.v a) + v (Some?.v b)
+  })
 = let open FStar.Integers in
   if (Some?a && Some? b && (Some?.v a) <= asn1_int32_max - (Some?.v b)) then
   ( Some (Some?.v a + Some?.v b) )
   else
   ( None )
+#pop-options
 
+private
+let serialize_asn1_value_of_type
+  (#_a: asn1_primitive_type)
+  (value: datatype_of_asn1_type _a)
+= match _a with
+  | BOOLEAN      -> serialize serialize_asn1_boolean value
+  | NULL         -> serialize serialize_asn1_null value
+  | OCTET_STRING -> let (|len, s|) = value <: datatype_of_asn1_type OCTET_STRING in
+                    let l = v len in
+                    serialize_asn1_octet_string_unfold l value;
+                    serialize (serialize_asn1_octet_string l) value
+
+let length_of_asn1_primitive_value_spec
+  (#_a: asn1_primitive_type)
+  (value: datatype_of_asn1_type _a)
+: GTot (length: asn1_length_t {
+       length == Seq.length (serialize_asn1_value_of_type value) /\
+       length == v (len_of_asn1_data _a value)
+  })
+= match _a with
+  | OCTET_STRING   -> let (|len, s|) = value <: datatype_of_asn1_type OCTET_STRING in
+                      let l = v len in
+                      serialize_asn1_octet_string_unfold l value;
+                      Seq.length (serialize_asn1_value_of_type value)
+  | NULL | BOOLEAN -> Seq.length (serialize_asn1_value_of_type value)
+
+#push-options "--query_stats --z3rlimit 32"
 let len_of_asn1_primitive_TLV
   (#_a: asn1_primitive_type)
-  (data: datatype_of_asn1_type _a)
-: Tot (x: option asn1_int32{Some? x ==> (I.v (Some?.v x) == Seq.length (serialize (serialize_asn1_TLV_of_type _a) data))})
-= let data_len = len_of_asn1_data _a data in
-  let len_len = len_of_asn1_length data_len in
-  let res = 1ul in
-  Some 1ul `safe_add` Some len_len `safe_add` Some data_len
+  (value: datatype_of_asn1_type _a)
+: Tot (len: option asn1_int32 {
+         Some? len ==>
+           (v (Some?.v len) == Seq.length (serialize (serialize_asn1_TLV_of_type _a) value))
+  })
+= (* Prf *) (match _a with
+             | BOOLEAN      -> (serialize_asn1_boolean_TLV_unfold (value <: datatype_of_asn1_type BOOLEAN))
+             | NULL         -> (serialize_asn1_null_TLV_unfold (value <: datatype_of_asn1_type NULL))
+             | OCTET_STRING -> (serialize_asn1_octet_string_TLV_unfold (value <: datatype_of_asn1_type OCTET_STRING)));
+  let value_len = len_of_asn1_data _a value in
+  (* Prf *) assert (v value_len == length_of_asn1_primitive_value_spec value);
 
-let parse_exact_bare
-  (#k: parser_kind)
-  (#t: Type0)
-  (p: parser k t)
-  (l: nat)
-: Tot (bare_parser t)
-= fun (input: bytes) ->
-  if (Seq.length input < l) then
-  ( None )
-  else
-  ( match parse p (Seq.slice input 0 l) with
-    | Some (v, n) -> if n = l then
-                     ( Some (v, (l <: consumed_length input)) )
-                     else
-                     ( None )
-    | None        -> None )
+  let len_len = len_of_asn1_length value_len in
 
-let parse_exact_bare_injective_prf
-  (#k: parser_kind)
-  (#t: Type0)
-  (p: parser k t)
-  (l: nat)
-  (input1: bytes)
-  (input2: bytes)
-: Lemma
-  (requires (injective_precond (parse_exact_bare p l) input1 input2))
-  (ensures (injective_postcond (parse_exact_bare p l) input1 input2))
-= if (Seq.length input1 < l) then
-  ( () )
-  else
-  ( match parse p (Seq.slice input1 0 l), parse p (Seq.slice input2 0 l) with
-    | Some (v1, n1), Some (v2, n2) -> if n1 = l && n2 = l then
-                                      ( parser_kind_prop_equiv k p;
-                                        assert (injective_postcond p (Seq.slice input1 0 l) (Seq.slice input2 0 l)) )
-                                      else
-                                      ( () )
-    | _        -> () )
+  let tag_len = 1ul in
 
-let parse_exact_bare_injective
-  (#k: parser_kind)
-  (#t: Type0)
-  (p: parser k t)
-  (l: nat)
-: Lemma (
-  injective (parse_exact_bare p l)
-)
-= Classical.forall_intro_2 (
-    fun (s1 s2: bytes) ->
-      Classical.move_requires_2 (parse_exact_bare_injective_prf p l) s1 s2
-  )
+  (* Prf *) assert (v tag_len + v len_len + v value_len == Seq.length (serialize (serialize_asn1_TLV_of_type _a) value));
 
-let parse_exact_kind
-  (#k: parser_kind)
-  (#t: Type0)
-  (p: parser k t)
-  (l: nat)
-: parser_kind = {
-  parser_kind_low = l;
-  parser_kind_high = Some l;
-  parser_kind_subkind = None;
-  parser_kind_metadata = None
-}
-
-let parse_exact_correct
-  (#k: parser_kind)
-  (#t: Type0)
-  (p: parser k t)
-  (l: nat)
-: Lemma (
-  parser_kind_prop (parse_exact_kind p l) (parse_exact_bare p l)
-)
-= parser_kind_prop_equiv (parse_exact_kind p l) (parse_exact_bare p l);
-  parse_exact_bare_injective p l
-
-let parse_exact
-  (#k: parser_kind)
-  (#t: Type0)
-  (p: parser k t)
-  (l: nat)
-: parser (parse_exact_kind p l) t
-= parse_exact_correct p l;
-  parse_exact_bare p l
+(* return *) Some tag_len `safe_add` Some len_len `safe_add` Some value_len
+#pop-options
 
 
 /// Example
@@ -188,7 +148,7 @@ let len_of_inner_t
   let len_s1 = len_of_asn1_primitive_TLV x.s1 in
   len_n1 `safe_add` len_s1
 
-let parse_inner
+let parse_inner_value
 : parser _ inner_t
 = parse_asn1_TLV_of_type NULL
   `nondep_then`
@@ -196,8 +156,8 @@ let parse_inner
   `parse_synth`
   synth_inner_t
 
-let serialize_inner
-: serializer parse_inner
+let serialize_inner_value
+: serializer parse_inner_value
 = serialize_synth
   (* p1 *) (parse_asn1_TLV_of_type NULL
             `nondep_then`
@@ -209,12 +169,56 @@ let serialize_inner
   (* g1 *) (synth_inner_t_inverse)
   (* Prf*) ()
 
-let parse_exact_kind_weak = {
-  parser_kind_low = asn1_length_min;
-  parser_kind_high = Some asn1_length_max;
-  parser_kind_subkind = None;
-  parser_kind_metadata = None
-}
+let parse_inner_sequence
+= parse_asn1_sequence_TLV serialize_inner_value
+
+let parse_inner_sequence_unfold
+= parse_asn1_sequence_TLV_unfold serialize_inner_value
+
+#restart-solver
+#push-options "--query_stats --z3rlimit 32"
+let parse_inner_sequence_test
+  ()
+=
+  let x = {
+    n1 = ();
+    s1 = (|3ul, Seq.create 3 9uy|)
+  } in
+  let raw_seq =
+    serialize (serialize_the_asn1_tag SEQUENCE) SEQUENCE
+    `Seq.append`
+    serialize (serialize_asn1_length_of_type SEQUENCE) (Some?.v (len_of_inner_t x))
+    // `Seq.append`
+    // serialize_asn1_null_TLV x.n1
+    // `Seq.append`
+    // serialize_asn1_octet_string_TLV x.s1
+  in
+  serialize_the_asn1_tag_unfold SEQUENCE SEQUENCE;
+  serialize_u8_spec (synth_the_asn1_tag_inverse SEQUENCE SEQUENCE);
+  serialize_u8_spec' (synth_the_asn1_tag_inverse SEQUENCE SEQUENCE);
+  serialize_asn1_length_of_type_unfold SEQUENCE (Some?.v (len_of_inner_t x));
+  serialize_asn1_null_TLV_unfold x.n1;
+  serialize_asn1_octet_string_TLV_unfold x.s1;
+
+  parse_inner_sequence_unfold raw_seq;
+  assert (raw_seq.[0] == (serialize (serialize_the_asn1_tag SEQUENCE) SEQUENCE).[0]);
+  parse_asn1_sequence_TL_unfold raw_seq;
+  parse_the_asn1_tag_unfold SEQUENCE raw_seq;
+  parse_u8_spec raw_seq;
+  parse_u8_spec' raw_seq;
+  assert (raw_seq.[0] == 0x30uy);
+  let px_raw = parse (parse_u8) raw_seq in
+  assert (Some? px_raw);
+  parse_u8_spec' raw_seq;
+
+  let px_t  = parse (parse_the_asn1_tag SEQUENCE) raw_seq in
+  assert (Some? px_t);
+
+  let px_tl = parse parse_asn1_sequence_TL raw_seq in
+  // let pseq = parse (parse_inner_sequence) raw_seq in
+  assert (Some? px_tl);
+
+()
 
 let lmm (b: bytes): Lemma
   (requires (Some? (parse parse_inner b)))
@@ -226,7 +230,7 @@ let lmm (b: bytes): Lemma
 let lm (): Lemma (
   let s = Seq.create 5 1uy in
   let i = {n1 = (); s1 = (|5ul, s|)} in
-  let pe = parse_exact parse_inner (I.v (Some?.v (len_of_inner_t i))) in
+  let pe = parse_exact parse_inner (v (Some?.v (len_of_inner_t i))) in
   let sx = serialize serialize_inner i in
   let px = parse pe sx in
   (Some? px) /\ (len_of_inner_t i) == Some 9ul
@@ -255,7 +259,7 @@ let parse_inner_TLV
 = let p = (fun (x: (the_asn1_type SEQUENCE * asn1_int32_of_type SEQUENCE)) ->
             // parse_exact_kind_weak
             // `weaken`
-            parse_exact parse_inner (I.v (snd x))) in
+            parse_exact parse_inner (v (snd x))) in
   // assume (and_then_cases_injective p);
   parse_tagged_union
   (* pt *) (parse_the_asn1_tag SEQUENCE
