src/asn1/ASN1.Low.OCTET_STRING.fst
@@ -13,32 +13,33 @@ module MB = LowStar.Monotonic.Buffer
 module B = LowStar.Buffer
 module Cast = FStar.Int.Cast
 
-let serialize32_asn1_octet_string
-  (len: size_t)
-: Tot (serializer32 (serialize_asn1_octet_string (v len)))
-= fun (s: lbytes_t (v len))
-    (#rrel #rel: _)
-    (b: B.mbuffer byte_t rrel rel)
-    (pos: size_t)
-->  store_seqbytes
-    (* src *) s
-    (* from*) 0ul
-    (* to  *) len
-    (* dst *) b
-    (* pos *) pos;
-(* retuen *) len
+// let serialize32_asn1_octet_string
+//   (len: size_t)
+// : Tot (serializer32 (serialize_asn1_octet_string (v len)))
+// = fun (value: datatype_of_asn1_type OCTET_STRING { v (dfst value) == v len })
+//     (#rrel #rel: _)
+//     (b: B.mbuffer byte_t rrel rel)
+//     (pos: size_t)
+// ->  store_seqbytes
+//     (* src *) (dsnd value)
+//     (* from*) 0ul
+//     (* to  *) len
+//     (* dst *) b
+//     (* pos *) pos;
+
+// (* retuen *) len
 
 let serialize32_asn1_octet_string_backwards
   (len: size_t)
 : Tot (serializer32_backwards (serialize_asn1_octet_string (v len)))
-= fun (s: lbytes_t (v len))
+= fun (value: datatype_of_asn1_type OCTET_STRING { v (dfst value) == v len })
     (#rrel #rel: _)
     (b: B.mbuffer byte_t rrel rel)
     (pos: size_t)
 ->  (* Prf *) let h0 = HST.get () in
 
     store_seqbytes
-    (* src *) s
+    (* src *) (dsnd value)
     (* from*) 0ul
     (* to  *) len
     (* dst *) b
