src/asn1/ASN1.Spec.BOOLEAN.fsti
@@ -98,7 +98,7 @@ val parse_asn1_boolean_TLV_unfold
        (let input_V = Seq.slice input_LV consumed_L (Seq.length input_LV) in
         match parse parse_asn1_boolean input_V with
         | None -> None
-        | Some (value, consumed_V) -> Some (value, consumed_T + consumed_L + consumed_V))))
+        | Some (value, consumed_V) -> Some (value, (consumed_T + consumed_L + consumed_V <: consumed_length input_TLV)))))
 )
 
 let serialize_asn1_boolean_TLV
