src/asn1/ASN1.Spec.NULL.fst
@@ -65,3 +65,75 @@ let serialize_asn1_null_TLV
             serialize_asn1_null)
   (* g1 *) (synth_asn1_null_TLV_inverse)
   (* Prf*) ()
+
+let parse_asn1_null_TLV_unfold
+  (input_TLV: bytes)
+: Lemma (
+  parse parse_asn1_null_TLV input_TLV ==
+ (match parse (parse_the_asn1_tag NULL) input_TLV with
+  | None -> None
+  | Some (NULL, consumed_T) ->
+    (let input_LV = Seq.slice input_TLV consumed_T (Seq.length input_TLV) in
+     match parse (parse_asn1_length_of_type NULL) input_LV with
+     | None -> None
+     | Some (0ul, consumed_L) ->
+       (let input_V = Seq.slice input_LV consumed_L (Seq.length input_LV) in
+        match parse parse_asn1_null input_V with
+        | None -> None
+        | Some (value, consumed_V) -> Some (value, (consumed_T + consumed_L + consumed_V <: consumed_length input_TLV)))))
+)
+= nondep_then_eq
+  (* p1 *) (parse_the_asn1_tag NULL)
+  (* p2 *) (parse_asn1_length_of_type NULL)
+  (* in *) (input_TLV);
+  nondep_then_eq
+  (* p1 *) (parse_the_asn1_tag NULL
+            `nondep_then`
+            parse_asn1_length_of_type NULL)
+  (* p2 *) (parse_asn1_null)
+  (* in *) (input_TLV);
+  parse_synth_eq
+  (* p1 *) (parse_the_asn1_tag NULL
+            `nondep_then`
+            parse_asn1_length_of_type NULL
+            `nondep_then`
+            parse_asn1_null)
+  (* f2 *) (synth_asn1_null_TLV)
+  (* in *) (input_TLV)
+
+let serialize_asn1_null_TLV_unfold
+  (value: datatype_of_asn1_type NULL)
+: Lemma (
+  serialize serialize_asn1_null_TLV value
+  `Seq.equal`
+ (serialize (serialize_the_asn1_tag NULL) NULL
+  `Seq.append`
+  serialize (serialize_asn1_length_of_type NULL) 0ul
+  `Seq.append`
+  serialize serialize_asn1_null value)
+)
+= serialize_nondep_then_eq
+  (* s1 *) (serialize_the_asn1_tag NULL)
+  (* s2 *) (serialize_asn1_length_of_type NULL)
+  (* in *) (NULL, 0ul);
+  serialize_nondep_then_eq
+  (* s1 *) (serialize_the_asn1_tag NULL
+            `serialize_nondep_then`
+            serialize_asn1_length_of_type NULL)
+  (* s2 *) (serialize_asn1_null)
+  (* in *) ((NULL, 0ul), value);
+  serialize_synth_eq
+  (* p1 *) (parse_the_asn1_tag NULL
+            `nondep_then`
+            parse_asn1_length_of_type NULL
+            `nondep_then`
+            parse_asn1_null)
+  (* f2 *) (synth_asn1_null_TLV)
+  (* s1 *) (serialize_the_asn1_tag NULL
+            `serialize_nondep_then`
+            serialize_asn1_length_of_type NULL
+            `serialize_nondep_then`
+            serialize_asn1_null)
+  (* g1 *) (synth_asn1_null_TLV_inverse)
+  (* Prf*) ()
+  (* in *) (value)
