src/asn1/ASN1.Spec.OCTET_STRING.fst
@@ -10,54 +10,76 @@ open ASN1.Spec.Length
 
 open FStar.Integers
 
-// let synth_asn1_octet_string
-//   (l: asn1_length_t)
-//   (ls: lbytes l)
-// : GTot (x: datatype_of_asn1_type OCTET_STRING{v (dfst x) == l})
-//   // (requires True)
-//   // (ensures fun x -> v (dfst x) == l)
-// = (|I.u l, ls|)
+let synth_asn1_octet_string
+  (l: asn1_length_t)
+  (ls: lbytes l)
+: GTot (value: datatype_of_asn1_type OCTET_STRING{v (dfst value) == l})
+= (|u l, ls|)
 
-// let synth_asn1_octet_string_inverse
-//   (l: asn1_length_t)
-//   (x: datatype_of_asn1_type OCTET_STRING{v (dfst x) == l})
-// : GTot (ls: lbytes l)
-//   // (requires v (dfst x) == l)
-//   // (ensures fun ls -> synth_asn1_octet_string l ls == x)
-// = dsnd x
+let synth_asn1_octet_string_inverse
+  (l: asn1_length_t)
+  (value: datatype_of_asn1_type OCTET_STRING{v (dfst value) == l})
+: GTot (ls: lbytes l{ value == synth_asn1_octet_string l ls })
+= dsnd value
 
 let parse_asn1_octet_string_kind (l: asn1_length_t) = total_constant_size_parser_kind l
 let parse_asn1_octet_string
   (l: asn1_length_t)
-// : parser (parse_asn1_octet_string_kind l) (x: datatype_of_asn1_type OCTET_STRING{v (dfst x) == l})
+: parser (parse_asn1_octet_string_kind l) (x: datatype_of_asn1_type OCTET_STRING{v (dfst x) == l})
 = parse_seq_flbytes l
-//   `parse_synth`
-//   synth_asn1_octet_string l
+  `parse_synth`
+ synth_asn1_octet_string l
+
+let parse_asn1_octet_string_unfold
+  (l: asn1_length_t)
+  (input: bytes)
+: Lemma (
+  parse (parse_asn1_octet_string l) input ==
+ (match parse (parse_seq_flbytes l) input with
+  | None -> None
+  | Some (ls, consumed) -> Some (synth_asn1_octet_string l ls, consumed)))
+= parse_synth_eq
+  (* p1 *) (parse_seq_flbytes l)
+  (* f2 *) (synth_asn1_octet_string l)
+  (* in *) (input)
 
 let serialize_asn1_octet_string
   (l: asn1_length_t)
-= serialize_seq_flbytes l
-// = serialize_synth
-//   (* p1 *) (parse_seq_flbytes l)
-//   (* f2 *) (synth_asn1_octet_string l)
-  // (* s1 *) (serialize_seq_flbytes l)
-//   (* g1 *) (synth_asn1_octet_string_inverse l)
-//   (* Prf*) ()
+: serializer (parse_asn1_octet_string l)
+= serialize_synth
+  (* p1 *) (parse_seq_flbytes l)
+  (* f2 *) (synth_asn1_octet_string l)
+  (* s1 *) (serialize_seq_flbytes l)
+  (* g1 *) (synth_asn1_octet_string_inverse l)
+  (* Prf*) ()
 
-let parse_asn1_octet_string_kind_weak = strong_parser_kind asn1_length_min asn1_length_max None
+let serialize_asn1_octet_string_unfold
+  (l: asn1_length_t)
+  (value: datatype_of_asn1_type OCTET_STRING{v (dfst value) == l})
+: Lemma (
+  serialize (serialize_asn1_octet_string l) value ==
+  serialize (serialize_seq_flbytes l) (synth_asn1_octet_string_inverse l value))
+= serialize_synth_eq
+  (* p1 *) (parse_seq_flbytes l)
+  (* f2 *) (synth_asn1_octet_string l)
+  (* s1 *) (serialize_seq_flbytes l)
+  (* g1 *) (synth_asn1_octet_string_inverse l)
+  (* Prf*) ()
+  (* in *) (value)
+
 let parse_asn1_octet_string_weak
   (l: asn1_length_t)
-: parser parse_asn1_octet_string_kind_weak _ //(datatype_of_asn1_type OCTET_STRING)
-= (parse_asn1_octet_string_kind_weak
-   `weaken`
-   parse_asn1_octet_string l)
+: parser (weak_kind_of_type SEQUENCE) (value: datatype_of_asn1_type OCTET_STRING{v (dfst value) == l})
+= weak_kind_of_type SEQUENCE
+  `weaken`
+  parse_asn1_octet_string l
 
 let serialize_asn1_octet_string_weak
   (l: asn1_length_t)
 : serializer (parse_asn1_octet_string_weak l)
-= (parse_asn1_octet_string_kind_weak
-   `serialize_weaken`
-   serialize_asn1_octet_string l)
+= weak_kind_of_type SEQUENCE
+  `serialize_weaken`
+  serialize_asn1_octet_string l
 
 /// Specialized TLV
 ///
@@ -76,66 +98,60 @@ let parser_tag_of_octet_string
 : GTot (the_asn1_type OCTET_STRING & asn1_int32_of_type OCTET_STRING)
 = (OCTET_STRING, dfst x)
 
-let synth_asn1_octet_string_data
-  (len: asn1_int32_of_type OCTET_STRING)
-  (x: the_asn1_type OCTET_STRING & asn1_int32_of_type OCTET_STRING{x == (OCTET_STRING, len)})
-  (s: lbytes (v len))
-: GTot (refine_with_tag parser_tag_of_octet_string x)
-= let value: datatype_of_asn1_type OCTET_STRING = (|len, s|) in
-  let y: refine_with_tag parser_tag_of_octet_string x = value in
-  y
+// let synth_asn1_octet_string_data
+//   (len: asn1_int32_of_type OCTET_STRING)
+//   (x: the_asn1_type OCTET_STRING & asn1_int32_of_type OCTET_STRING{x == (OCTET_STRING, len)})
+//   (s: lbytes (v len))
+// : GTot (refine_with_tag parser_tag_of_octet_string x)
+// = let value: datatype_of_asn1_type OCTET_STRING = (|len, s|) in
+//   let y: refine_with_tag parser_tag_of_octet_string x = value in
+//   y
 
-let synth_asn1_octet_string_data_inverse
-  (len: asn1_int32_of_type OCTET_STRING)
-  (x: the_asn1_type OCTET_STRING & asn1_int32_of_type OCTET_STRING{x == (OCTET_STRING, len)})
-  (value: refine_with_tag parser_tag_of_octet_string x)
-: GTot (s: lbytes (v len))
-= dsnd
-    #(asn1_int32_of_type OCTET_STRING)
-    #(fun (len:asn1_int32_of_type OCTET_STRING) -> s:bytes{Seq.length s == v len})
-    value
+// let synth_asn1_octet_string_data_inverse
+//   (len: asn1_int32_of_type OCTET_STRING)
+//   (x: the_asn1_type OCTET_STRING & asn1_int32_of_type OCTET_STRING{x == (OCTET_STRING, len)})
+//   (value: refine_with_tag parser_tag_of_octet_string x)
+// : GTot (s: lbytes (v len))
+// = dsnd
+//     #(asn1_int32_of_type OCTET_STRING)
+//     #(fun (len:asn1_int32_of_type OCTET_STRING) -> s:bytes{Seq.length s == v len})
+//     value
 
-let parse_asn1_octet_string_kind_strong
-  (x: the_asn1_type OCTET_STRING & asn1_int32_of_type OCTET_STRING)
-: parser_kind
-= total_constant_size_parser_kind (v (snd x))
+// let parse_asn1_octet_string_kind_strong
+//   (x: the_asn1_type OCTET_STRING & asn1_int32_of_type OCTET_STRING)
+// : parser_kind
+// = total_constant_size_parser_kind (v (snd x))
 
-let parse_asn1_octet_string_data
-  (x: the_asn1_type OCTET_STRING & asn1_int32_of_type OCTET_STRING)
-: Tot (parser (parse_asn1_octet_string_kind_strong x) (refine_with_tag parser_tag_of_octet_string x))
-= parse_asn1_octet_string (v (snd x))
-  `parse_synth`
-  synth_asn1_octet_string_data (snd x) x
+// let parse_asn1_octet_string_data
+//   (x: the_asn1_type OCTET_STRING & asn1_int32_of_type OCTET_STRING)
+// : Tot (parser (parse_asn1_octet_string_kind_strong x) (refine_with_tag parser_tag_of_octet_string x))
+// = parse_asn1_octet_string (v (snd x))
+//   `parse_synth`
+//   synth_asn1_octet_string_data (snd x) x
 
-let parse_asn1_octet_string_data_unfold
-  (input: bytes)
-: Lemma (
-  forall (x: the_asn1_type OCTET_STRING & asn1_int32_of_type OCTET_STRING).
-)
+// let serialize_asn1_octet_string_data
+//   (x: the_asn1_type OCTET_STRING & asn1_int32_of_type OCTET_STRING)
+// : Tot (serializer (parse_asn1_octet_string_data x))
+// = serialize_synth
+//   (* p1 *) (parse_asn1_octet_string (v (snd x)))
+//   (* f2 *) (synth_asn1_octet_string_data (snd x) x)
+//   (* s1 *) (serialize_asn1_octet_string (v (snd x)))
+//   (* g1 *) (synth_asn1_octet_string_data_inverse (snd x) x)
+//   (* Prf*) ()
 
-let serialize_asn1_octet_string_data
-  (x: the_asn1_type OCTET_STRING & asn1_int32_of_type OCTET_STRING)
-: Tot (serializer (parse_asn1_octet_string_data x))
-= serialize_synth
-  (* p1 *) (parse_asn1_octet_string (v (snd x)))
-  (* f2 *) (synth_asn1_octet_string_data (snd x) x)
-  (* s1 *) (serialize_asn1_octet_string (v (snd x)))
-  (* g1 *) (synth_asn1_octet_string_data_inverse (snd x) x)
-  (* Prf*) ()
+// let parse_asn1_octet_string_data_weak
+//   (x: the_asn1_type OCTET_STRING & asn1_int32_of_type OCTET_STRING)
+// : Tot (parser parse_asn1_octet_string_kind_weak (refine_with_tag parser_tag_of_octet_string x))
+// = parse_asn1_octet_string_kind_weak
+//   `weaken`
+//   parse_asn1_octet_string_data x
 
-let parse_asn1_octet_string_data_weak
-  (x: the_asn1_type OCTET_STRING & asn1_int32_of_type OCTET_STRING)
-: Tot (parser parse_asn1_octet_string_kind_weak (refine_with_tag parser_tag_of_octet_string x))
-= parse_asn1_octet_string_kind_weak
-  `weaken`
-  parse_asn1_octet_string_data x
-
-let serialize_asn1_octet_string_data_weak
-  (x: the_asn1_type OCTET_STRING & asn1_int32_of_type OCTET_STRING)
-: Tot (serializer (parse_asn1_octet_string_data_weak x))
-= parse_asn1_octet_string_kind_weak
-  `serialize_weaken`
-  serialize_asn1_octet_string_data x
+// let serialize_asn1_octet_string_data_weak
+//   (x: the_asn1_type OCTET_STRING & asn1_int32_of_type OCTET_STRING)
+// : Tot (serializer (parse_asn1_octet_string_data_weak x))
+// = parse_asn1_octet_string_kind_weak
+//   `serialize_weaken`
+//   serialize_asn1_octet_string_data x
 
 // let parse_asn1_octet_string_TLV_kind
 // = parse_asn1_tag_kind
@@ -150,7 +166,64 @@ let parse_asn1_octet_string_TLV_kind
   `and_then_kind`
   parse_asn1_length_kind_of_type OCTET_STRING
   `and_then_kind`
-  parse_asn1_octet_string_kind_weak
+  weak_kind_of_type SEQUENCE
+
+let synth_asn1_octet_string_V
+  (tag: (the_asn1_type OCTET_STRING & asn1_int32_of_type OCTET_STRING))
+  (value: datatype_of_asn1_type OCTET_STRING { v (dfst value) == v (snd tag) })
+: GTot (value': refine_with_tag parser_tag_of_octet_string tag)
+= value
+
+let synth_asn1_octet_string_V_inverse
+  (tag: (the_asn1_type OCTET_STRING & asn1_int32_of_type OCTET_STRING))
+  (value': refine_with_tag parser_tag_of_octet_string tag)
+: GTot (value: datatype_of_asn1_type OCTET_STRING { v (dfst value) == v (snd tag) /\ value' == synth_asn1_octet_string_V tag value})
+= value'
+
+let parse_asn1_octet_string_V
+  (tag: (the_asn1_type OCTET_STRING & asn1_int32_of_type OCTET_STRING))
+: parser (weak_kind_of_type SEQUENCE) (refine_with_tag parser_tag_of_octet_string tag)
+= parse_asn1_octet_string_weak (v (snd tag))
+  `parse_synth`
+  synth_asn1_octet_string_V tag
+
+let parse_asn1_octet_string_V_unfold
+  (tag: (the_asn1_type OCTET_STRING & asn1_int32_of_type OCTET_STRING))
+  (input: bytes)
+: Lemma (
+  parse (parse_asn1_octet_string_V tag) input ==
+ (match parse (parse_asn1_octet_string (v (snd tag))) input with
+  | None -> None
+  | Some (value, consumed) ->  Some (synth_asn1_octet_string_V tag value, consumed)))
+= parse_synth_eq
+  (* p1 *) (parse_asn1_octet_string_weak (v (snd tag)))
+  (* f2 *) (synth_asn1_octet_string_V tag)
+  (* in *) input
+
+let serialize_asn1_octet_string_V
+  (tag: (the_asn1_type OCTET_STRING & asn1_int32_of_type OCTET_STRING))
+: serializer (parse_asn1_octet_string_V tag)
+= serialize_synth
+  (* p1 *) (parse_asn1_octet_string_weak (v (snd tag)))
+  (* f2 *) (synth_asn1_octet_string_V tag)
+  (* s1 *) (serialize_asn1_octet_string_weak (v (snd tag)))
+  (* g1 *) (synth_asn1_octet_string_V_inverse tag)
+  (* prf*) ()
+
+let serialize_asn1_octet_string_V_unfold
+  (tag: (the_asn1_type OCTET_STRING & asn1_int32_of_type OCTET_STRING))
+  (value: refine_with_tag parser_tag_of_octet_string tag)
+: Lemma (
+  serialize (serialize_asn1_octet_string_V tag) value ==
+  serialize (serialize_asn1_octet_string (v (snd tag))) value
+)
+= serialize_synth_eq
+  (* p1 *) (parse_asn1_octet_string_weak (v (snd tag)))
+  (* f2 *) (synth_asn1_octet_string_V tag)
+  (* s1 *) (serialize_asn1_octet_string_weak (v (snd tag)))
+  (* g1 *) (synth_asn1_octet_string_V_inverse tag)
+  (* prf*) ()
+  (* in *) (value)
 
 let parse_asn1_octet_string_TLV
 : parser parse_asn1_octet_string_TLV_kind (datatype_of_asn1_type OCTET_STRING)
@@ -159,33 +232,50 @@ let parse_asn1_octet_string_TLV
             `nondep_then`
             parse_asn1_length_of_type OCTET_STRING)
   (* tg *) (parser_tag_of_octet_string)
-  (* p  *) (parse_asn1_octet_string_data_weak)
+  (* p  *) (parse_asn1_octet_string_V)
 
+#restart-solver
+#push-options "--query_stats --z3rlimit 16 --initial_fuel 8"
 let parse_asn1_octet_string_TLV_unfold
   (input: bytes)
 : Lemma (
   parse parse_asn1_octet_string_TLV input ==
  (match parse (parse_the_asn1_tag OCTET_STRING) input with
   | None -> None
-  | Some (v_T, l_T) ->
-    (let input_LV = Seq.slice input l_T (Seq.length input) in
+  | Some (tag, consumed_tag) ->
+    (let input_LV = Seq.slice input consumed_tag (Seq.length input) in
      match parse (parse_asn1_length_of_type OCTET_STRING) input_LV with
      | None -> None
-     | Some (v_L, l_L) ->
-       (let input_data = Seq.slice input_LV l_L (Seq.length input_LV) in
-        match parse (parse_asn1_octet_string_data (v_T, v_L)) input_data with
+     | Some (len, consumed_len) ->
+       (let input_V = Seq.slice input_LV consumed_len (Seq.length input_LV) in
+        match parse (parse_asn1_octet_string_V (tag, len)) input_V with
         | None -> None
-        | Some (v_V, l_V) -> Some (v_V, (l_T + l_L + l_V <: consumed_length input)))
+        | Some (value, consumed_value) -> Some (value, (consumed_tag + consumed_len + consumed_value <: consumed_length input)))
      ))
 )
 = nondep_then_eq
   (* p1 *) (parse_the_asn1_tag OCTET_STRING)
   (* p2 *) (parse_asn1_length_of_type OCTET_STRING)
   (* in *) (input);
-  parse_synth_eq
-  (* p1 *) (parse_asn1_octet_string (v (snd x)))
-  (* f2 *) (synth_asn1_octet_string_data)
-  (* in *)
+
+  let parsed_tag
+  = parse (parse_the_asn1_tag OCTET_STRING
+           `nondep_then`
+           parse_asn1_length_of_type OCTET_STRING) input in
+  if (Some? parsed_tag) then
+  ( let Some (tag, consumed) = parsed_tag in
+    parse_asn1_octet_string_V_unfold tag input );
+
+  parse_tagged_union_eq
+  (* pt *) (parse_the_asn1_tag OCTET_STRING
+            `nondep_then`
+            parse_asn1_length_of_type OCTET_STRING)
+  (* tg *) (parser_tag_of_octet_string)
+  (* p  *) (fun tag -> parse_asn1_octet_string_V_unfold tag input;
+                     parse_asn1_octet_string_V tag)
+  (* in *) (input)
+
+#pop-options
 
 let serialize_asn1_octet_string_TLV
 : serializer parse_asn1_octet_string_TLV
@@ -194,14 +284,50 @@ let serialize_asn1_octet_string_TLV
             `serialize_nondep_then`
             serialize_asn1_length_of_type OCTET_STRING)
   (* tg *) (parser_tag_of_octet_string)
-  (* s  *) (serialize_asn1_octet_string_data_weak)
+  (* s  *) (serialize_asn1_octet_string_V)
+  // (* s  *) (fun (tag: (the_asn1_type OCTET_STRING & asn1_int32_of_type OCTET_STRING))
+  //           -> serialize_synth
+  //              (* p1 *) (parse_asn1_octet_string_weak (v (snd tag)))
+  //              (* f2 *) (fun value -> value <: refine_with_tag parser_tag_of_octet_string tag)
+  //              (* s1 *) (serialize_asn1_octet_string_weak (v (snd tag)))
+  //              (* g1 *) (fun value -> value <: value: datatype_of_asn1_type OCTET_STRING{v (dfst value) == v (snd tag)})
+  //              (* prf*) ())
 
-let length_lemma
-  (input: bytes)
-: Lemma
-  (requires (Some? (parse parse_asn1_octet_string_TLV input)))
-  (ensures (
-    let px = parse parse_asn1_octet_string_TLV input in
-    let pt = parse (parse_the_asn1_tag OCTET_STRING) input in
-    let pl = parse (parse_asn1_length_of_type OCTET_STRING) (Seq.slice input 0 )
-  ))
+#push-options "--query_stats --z3rlimit 32"
+let serialize_asn1_octet_string_TLV_unfold
+  (value: datatype_of_asn1_type OCTET_STRING)
+: Lemma (
+  serialize serialize_asn1_octet_string_TLV value ==
+  serialize (serialize_the_asn1_tag OCTET_STRING) OCTET_STRING
+  `Seq.append`
+  serialize (serialize_asn1_length_of_type OCTET_STRING) (dfst value)
+  `Seq.append`
+  serialize (serialize_asn1_octet_string_weak (v (dfst value))) value
+)
+= serialize_nondep_then_eq
+  (* s1 *) (serialize_the_asn1_tag OCTET_STRING)
+  (* s2 *) (serialize_asn1_length_of_type OCTET_STRING)
+  (* in *) (parser_tag_of_octet_string value);
+  serialize_asn1_octet_string_V_unfold (parser_tag_of_octet_string value) value;
+  serialize_tagged_union_eq
+  (* st *) (serialize_the_asn1_tag OCTET_STRING
+            `serialize_nondep_then`
+            serialize_asn1_length_of_type OCTET_STRING)
+  (* tg *) (parser_tag_of_octet_string)
+  (* s  *) (serialize_asn1_octet_string_V)
+  (* in *) (value)
+#pop-options
+
+private
+let length_test
+  (value: datatype_of_asn1_type OCTET_STRING)
+: Lemma (
+  let (|len, s|) = value in
+  v len == Seq.length (serialize (serialize_asn1_octet_string (v (snd (parser_tag_of_octet_string value)))) value)
+)
+= let tag = parser_tag_of_octet_string value in
+  let l = v (snd tag) in
+  parser_kind_prop_equiv
+  (* k *) (parse_asn1_octet_string_kind l)
+  (* p *) (parse_asn1_octet_string l);
+  serialize_asn1_octet_string_unfold l value
